Add length bound in AlignedIPChecksum

src/Narcissus/BinLib/AlignedIPChecksum.v
@@ -43,16 +43,38 @@ Definition IPChecksum (b b' : ByteString) : ByteString :=
           (encode_word (wnot (onesComplement
                                 (ByteString2ListOfChar (bin_measure (mappend b b')) (BoundedByteStringToByteString(mappend b b')))))).
 
-Fixpoint Vector_checksum_bound n {sz} (bytes :Vector.t (word 8) sz) : InternetChecksum.W16 :=
+Fixpoint Vector_checksum_bound n {sz} (bytes :Vector.t (word 8) sz) acc : InternetChecksum.W16 :=
   match n, bytes with
-  | 0, _ => wzero _
-  | S 0, Vector.nil => InternetChecksum.add_bytes_into_checksum (wzero _) (wzero _) (wzero _)
-  | S 0, Vector.cons x _ _ => InternetChecksum.add_bytes_into_checksum x (wzero _) (wzero _)
-  | S (S n'), Vector.cons x _ Vector.nil => InternetChecksum.add_bytes_into_checksum x (wzero _) (Vector_checksum_bound n' (Vector.nil _))
-  | S (S n'), Vector.nil => InternetChecksum.add_bytes_into_checksum (wzero _) (wzero _)
-                                                                     (Vector_checksum_bound n' (Vector.nil _))
-  | S (S n'), Vector.cons x _ (Vector.cons y _ t) => InternetChecksum.add_bytes_into_checksum x y (Vector_checksum_bound n' t)
+  | 0, _ => acc
+  | _, Vector.nil => acc
+  | S 0, Vector.cons x _ _ => InternetChecksum.add_bytes_into_checksum x (wzero _) acc
+  | _, Vector.cons x _ Vector.nil => InternetChecksum.add_bytes_into_checksum x (wzero _) acc
+  | S (S n'), Vector.cons x _ (Vector.cons y _ t) =>
+    (Vector_checksum_bound n' t (InternetChecksum.add_bytes_into_checksum x y acc))
   end.
+
+Definition Vector_checksum_bound' n {sz} (bytes : Vector.t (word 8) sz) : InternetChecksum.W16 :=
+  InternetChecksum.Vector_fold_left_pair InternetChecksum.add_bytes_into_checksum n bytes (wzero _) (wzero _).
+
+Lemma Vector_checksum_bound'_ok' :
+  forall n {sz} (bytes :Vector.t (word 8) sz) acc,
+    Vector_checksum_bound n bytes acc =
+    InternetChecksum.Vector_fold_left_pair InternetChecksum.add_bytes_into_checksum n bytes acc (wzero _).
+Proof.
+  fix IH 3.
+  destruct bytes as [ | hd sz [ | hd' sz' tl ] ]; intros; simpl.
+  - destruct n as [ | [ | ] ]; reflexivity.
+  - destruct n as [ | [ | ] ]; reflexivity.
+  - destruct n as [ | [ | ] ]; simpl; try reflexivity.
+    rewrite IH; reflexivity.
+Qed.
+
+Lemma Vector_checksum_bound'_ok :
+  forall n {sz} (bytes :Vector.t (word 8) sz),
+    Vector_checksum_bound n bytes (wzero _) = Vector_checksum_bound' n bytes.
+Proof.
+  intros; apply Vector_checksum_bound'_ok'.
+Qed.
 
 Definition IPChecksum_Valid_dec (n : nat) (b : ByteString)
   : {IPChecksum_Valid' n b} + {~IPChecksum_Valid' n b} := weq _ _.
@@ -96,7 +118,7 @@ Lemma CorrectAlignedDecoderForIPChecksumThenC {A}
          (format_A ThenChecksum IPChecksum_Valid' OfSize 16 ThenCarryOn format_B).
 Proof.
   intros H; destruct H as [ ? [ [? ?] [ ? ?] ] ]; simpl in *.
-  eexists (fun sz v => if weq (Vector_checksum_bound 20 v) (wones 16) then x sz v  else ThrowAlignedDecodeM v).
+  eexists (fun sz v => if weq (Vector_checksum_bound' 20 v) (wones 16) then x sz v  else ThrowAlignedDecodeM v).
   admit.
 Defined.
 
@@ -169,7 +191,7 @@ Lemma CorrectAlignedDecoderForUDPChecksumThenC {A}
          (format_A ThenChecksum (Pseudo_Checksum_Valid srcAddr destAddr udpLength protoCode) OfSize 16 ThenCarryOn format_B).
 Proof.
   intros H; destruct H as [ ? [ [? ?] [ ? ?] ] ]; simpl in *.
-  eexists (fun sz v => if weq (Vector_checksum_bound (96 + sz * 8)
+  eexists (fun sz v => if weq (Vector_checksum_bound' (96 + sz * 8)
                                                      (Vector.cons _ (wzero 8) _ (Vector.cons _ protoCode _
                                                                       (append v (append srcAddr (append destAddr udpLength)))))) (wones 16)
                                                      
